Cedille/Lemma/Confluence.lean
@@ -1,0 +1,8 @@
+
+import Cedille.Def
+
+namespace Cedille
+
+  theorem confluence : t -β>* t1 -> t -β>* t2 -> ∃ z, t1 -β>* z ∧ t2 -β>* z := sorry
+
+end Cedille
