Cedille/Lemma/Red.lean
@@ -1,7 +1,11 @@
 
 import Cedille.Def
+import Cedille.Lemma.Refold
+import Cedille.Lemma.Erasure
 
 namespace Cedille
+
+  lemma red_pi : A -β>* A' -> B -β>* B' -> pi m A B -β>* pi m A' B' := sorry
 
   lemma red_pi1 : A -β>* A' -> pi m A B -β>* pi m A' B := sorry
 
@@ -19,29 +23,46 @@ namespace Cedille
 
   lemma red_inter2 : {_|-> x}B -β>* B' -> inter A B -β>* inter A ({_<-| x}B') := sorry
 
-  lemma red_pair1 : t -β>* t' -> pair t s -β>* pair t' s := sorry
+  lemma red_pair1 : t -β>* t' -> pair t s a -β>* pair t' s a := sorry
 
   lemma red_fst : t -β>* t' -> fst t -β>* fst t' := sorry
 
   lemma red_snd : t -β>* t' -> snd t -β>* snd t' := sorry
 
-  lemma red_eq1 : a -β>* a' -> eq a b -β>* eq a' b := sorry
+  lemma red_eq1 : a -β>* a' -> eq A a b -β>* eq A a' b := sorry
 
-  lemma red_eq2 : b -β>* b' -> eq a b -β>* eq a b' := sorry
+  lemma red_eq2 : b -β>* b' -> eq A a b -β>* eq A a b' := sorry
 
   lemma red_promote : t -β>* t' -> promote t -β>* promote t' := sorry
 
   lemma red_phi : a -β>* a' -> phi a b e -β>* phi a' b e := sorry
 
-  lemma red_delta : t -β>* t' -> delta t -β>* delta t' := sorry
+  lemma red_deltatop : t -β>* t' -> deltatop t -β>* deltatop t' := sorry
 
   lemma red_open_erase : {_|-> x}(erase t) -β> s -> erase ({_|-> x}t) -β> s := sorry
 
-  namespace RedStar
+  lemma red_strictify_erasure :
+    erase ({_|-> Name.fresh S1}t) -β> s ->
+    erase ({_|-> Name.fresh (S1 ++ S2)}t) -β> s
+  := sorry
 
-    lemma transitive : a -β>* b -> b -β>* c -> a -β>* c := sorry
+  lemma red_open_close : A -β>* {_|-> x}B -> ({_<-| x}A) -β>* B := sorry
+
+  namespace RedStar
+    lemma trans : a -β>* b -> b -β>* c -> a -β>* c := by {
+      intros h1 h2
+      induction h1 generalizing c
+      case refl a' => simp [*]
+      case step t1 t2 t3 s1 _s2 ih => {
+        have lem := ih h2
+        apply RedStar.step s1 lem
+      }
+    }
 
   end RedStar
 
+  lemma ctt_normal : ¬ (ctt -β> t) := sorry
+  lemma cff_normal : ¬ (cff -β> t) := sorry
+  lemma cbool_normal : ¬ (cbool -β> t) := sorry
 
 end Cedille
