Cedille/Lemma/RedErasure.lean
@@ -1,0 +1,94 @@
+
+import Cedille.Def
+import Cedille.Lemma.Refold
+import Cedille.Lemma.Erasure
+import Cedille.Lemma.Red
+
+namespace Cedille
+
+  lemma red_erasure_step :
+    erase t1 = erase t2 ->
+    t1 -β> z1 ->
+    ∃ z2, t2 -β>* z2 ∧ erase z1 = erase z2
+  := λ h step => @Nat.subInduction
+    (λ n1 n2 =>
+      (t1 t2 z1 : _) ->
+      size t1 ≤ n1  ->
+      size t2 ≤ n2 ->
+      erase t1 = erase t2 ->
+      t1 -β> z1 ->
+      ∃ z2, t2 -β>* z2 ∧ erase z1 = erase z2)
+    (by {
+      intros m t1 t2 z1 h1 h2 e step
+      have lem : size t1 = 0 := sorry
+      cases t1 <;> simp at lem <;> cases step
+    })
+    (by {
+      intros n t1 t2 z1 h1 h2 e step
+      sorry
+    })
+    (by {
+      intros n m ih t1 t2 z1 h1 h2 e step
+      cases t1 <;> cases t2 <;> simp at * <;> simp
+      case bound.bound _ => cases step
+      case bound.free _ => cases step
+      case bound.const _ => cases step
+      case bound.bind _ => cases step
+      case bound.ctor _ => cases step
+      case free.bound _ => cases step
+      case free.free _ => cases step
+      case free.const _ => cases step
+      case free.bind _ => cases step
+      case free.ctor _ => cases step
+      case const.bound _ => cases step
+      case const.free _ => cases step
+      case const.const _ => cases step
+      case const.bind _ => cases step
+      case const.ctor _ => cases step
+      case bind.bound _ q1 qstep k u1 u2 i => {
+        cases k
+        case lam m => {
+          cases m <;> simp at * <;> simp [*]
+        }
+        case pi m => {
+
+        }
+        case inter => {
+
+        }
+      }
+    })
+    (size t1)
+    (size t2)
+    t1
+    t2
+    z1
+    (by simp)
+    (by simp)
+    h
+    step
+
+
+
+  lemma red_erasure :
+    erase t1 = erase t2 ->
+    t1 -β>* z1 ->
+    ∃ z2, t2 -β>* z2 ∧ erase z1 = erase z2
+  := by {
+    intro h step
+    induction step generalizing t2
+    case refl t' => {
+      exists t2; simp [*]
+      apply RedStar.refl
+    }
+    case step u1 u2 u3 s1 _s2 e => {
+      have lem := red_erasure_step h s1
+      casesm* ∃ _, _, _ ∧ _; case _ w step e2 =>
+      have lem := @e w e2
+      casesm* ∃ _, _, _ ∧ _; case _ w' step' e3 =>
+      exists w'; simp [*]
+      apply RedStar.trans step step'
+    }
+  }
+
+end Cedille
