Cedille/Lemma/Rule.lean
@@ -1,0 +1,53 @@
+
+import Cedille.Def
+import Cedille.Lemma.Conv
+
+namespace Cedille
+
+  lemma infer_implies_cinfer : Γ ⊢ t : A -> Γ ⊢ t >: A := by {
+    intro j; apply ConInfer.infer j RedStar.refl
+  }
+
+  lemma infer_implies_check : Γ ⊢ t : A -> Γ ⊢ t =: A := by {
+    intro j; apply Check.check j Conv.refl
+  }
+
+  lemma infer_implies_wf : Γ ⊢ t : A -> ⊢ Γ := sorry
+
+  lemma cinfer_implies_check : Γ ⊢ t >: A -> Γ ⊢ t =: A := by {
+    intro j; cases j
+    case _ A' j step =>
+    apply Check.check j _
+    apply Conv.red_b Conv.refl step
+  }
+
+  lemma check_from_cinfer :
+    Γ ⊢ t >: A ->
+    A =β= B ->
+    Γ ⊢ t =: B
+  := by {
+    intros j e
+    cases j
+    case _ C j step =>
+    have lem := Conv.red_b e step
+    apply Check.check j lem
+  }
+
+  lemma cinfer_destruct : Γ ⊢ t >: B -> ∃ A, Γ ⊢ t : A ∧ A -β>* B := by {
+    intros j; cases j
+    case _ B j step => exists B
+  }
+
+  lemma rename_ctx_invariant {Γ : Map! Term} : (y : Name) -> x ∉ Map.fv Γ -> [x |-> y]Γ = Γ
+  := sorry
+
+  lemma rename_term_invariant {A : Term} : (y : Name) -> x ∉ fv A -> {_|-> y}{_<-| x}A = A
+  := sorry
+
+  lemma rename_infer (x : Name) :
+    Γ ⊢ t : A ->
+    y ∉ (Map.fv Γ ++ fv t ++ fv A) ->
+    [x |-> y]Γ ⊢ {_|-> y}{_<-| x}t : {_|-> y}{_<-| x}A
+  := sorry
+
+end Cedille
